Compilation_Alt.thy
@@ -1,0 +1,5 @@
+theory Compilation_Alt
+  imports Temporal_Plans
+begin
+
+end
