PDDL_temporal_plan_instantiation.thy
@@ -1,0 +1,18 @@
+theory PDDL_temporal_plan_instantiation
+  imports Temporal_AI_Planning_Languages_Semantics.TEMPORAL_PDDL_Semantics
+    Temporal_Plans
+    Containers.Containers
+begin
+
+derive (linorder) compare rat
+
+derive (eq) ceq predicate func atom object formula 
+derive ccompare predicate func atom object formula
+derive (no) cenum atom object formula
+derive (rbt) set_impl func atom object formula
+
+derive (rbt) mapping_impl object
+
+derive linorder predicate func object atom "object atom formula"
+
+end
